working towards induct lemma, aux state.

SimAsm/SimAsm_StateStack.thy
@@ -26,15 +26,47 @@ record ('var,'val) frame =
   frame_st :: "'var \<Rightarrow> 'val option" 
   frame_cap :: "'var set" 
 
-type_synonym ('var,'val) stack = "('var, 'val) frame list" 
+type_synonym ('var,'val,'a) stack = "('var, 'val,'a) frame_scheme list" 
 
-abbreviation Pred_tstack :: "('var,'val) stack \<Rightarrow> bool" where 
-  "Pred_tstack t \<equiv> t \<noteq> [] \<and> frame_cap (last t) = UNIV \<and> (\<forall>v. frame_st (last t) v \<noteq> None)"
+definition Is_tstack :: "('var,'val,'a) stack \<Rightarrow> bool" where 
+  "Is_tstack t \<equiv> t \<noteq> [] \<and> frame_cap (last t) = UNIV \<and> (\<forall>v. frame_st (last t) v \<noteq> None)"
 
-typedef ('var,'val) tstack = "{t :: ('var,'val) stack. Pred_tstack t}"
+lemma Is_tstack_ConsI [intro]: "Is_tstack xs \<Longrightarrow> Is_tstack (x#xs)" 
+  unfolding Is_tstack_def  
+  by auto
+
+lemma Is_tstack_ConsE [intro]: "xs \<noteq> [] \<Longrightarrow> Is_tstack (x#xs) \<Longrightarrow> Is_tstack xs" 
+  unfolding Is_tstack_def  
+  by auto                           
+
+lemma Is_tstack_NilE [elim!,dest!]: "Is_tstack [] \<Longrightarrow> False" 
+  unfolding Is_tstack_def
+  by auto  
+
+lemma Is_tstackE [elim,dest]:
+  assumes "Is_tstack s"  
+  shows "s \<noteq> []" "x \<in> frame_cap (last s)" "frame_st (last s) v \<noteq> None" 
+using assms
+unfolding Is_tstack_def
+by auto
+
+lemma Is_tstack_notcap [intro]: 
+  assumes "v \<notin> frame_cap x" "Is_tstack (x#xs)"
+  shows "Is_tstack xs" 
+proof - 
+  have "xs \<noteq> []" using assms unfolding Is_tstack_def by auto
+  thus ?thesis using assms unfolding Is_tstack_def by simp
+qed
+
+lemma Is_tstack_baseNone [intro]: "frame_st s v = None \<Longrightarrow> Is_tstack [s] \<Longrightarrow> False"
+  unfolding Is_tstack_def
+  by (metis last_ConsL)  
+  
+typedef ('var,'val,'a) tstack = "{t :: ('var,'val,'a) stack. Is_tstack t}"
+unfolding Is_tstack_def
 proof (standard, clarify, intro conjI allI)
-  fix x
-  let ?f = "\<lparr>frame_st = \<lambda>_. Some x, frame_cap = UNIV\<rparr> :: ('var,'val) frame" 
+  fix x a
+  let ?f = "\<lparr>frame_st = \<lambda>_. Some x, frame_cap = UNIV, \<dots> = a\<rparr> :: ('var,'val,'a) frame_scheme" 
   have last: "last [?f] = ?f" using last_ConsL by fast
   show "[?f] \<noteq> []" by fast
   show "frame_st (last [?f]) v \<noteq> None" for v
@@ -43,70 +75,128 @@ proof (standard, clarify, intro conjI allI)
     unfolding last select_convs(2) by simp
 qed
 
-abbreviation Is_tstack where 
-  "Is_tstack fs \<equiv> Pred_tstack (Rep_tstack fs)"
+(* declare Abs_tstack_inverse[intro] *)
 
-fun lookup :: "('var,'val) stack \<Rightarrow> 'var \<Rightarrow> 'val" where 
+abbreviation RepAbs_tstack where 
+  "RepAbs_tstack s \<equiv> Rep_tstack (Abs_tstack s)"
+
+lemma RepAbs_id [intro,simp]:
+  "Is_tstack s \<Longrightarrow> RepAbs_tstack s = s" 
+by (auto intro: Abs_tstack_inverse)
+
+lemma Rep_tstackI [intro!]:
+  shows 
+    "Rep_tstack s \<noteq> []" 
+    "x \<in> frame_cap (last (Rep_tstack s))" 
+    "frame_st (last (Rep_tstack s)) v \<noteq> None" 
+by (induct s) (auto simp add: Abs_tstack_inverse)
+
+lemma Is_tstack_induct [case_names Base Frame Is_tstack]:
+assumes "\<And>x. Is_tstack [x] \<Longrightarrow> P [x]"
+assumes "\<And>x xs. P xs \<Longrightarrow> Is_tstack xs \<Longrightarrow> P (x#xs)"
+assumes "Is_tstack s"
+shows "P s"
+using assms
+proof (induct s)
+  case (Cons a s)
+  thus ?case 
+  by (cases s) (auto intro: assms)
+qed auto
+
+lemma tstack_induct [case_names Base Frame]: 
+assumes "\<And>x. Is_tstack [x] \<Longrightarrow> P (Abs_tstack [x])"
+assumes "\<And>x xs. P (Abs_tstack xs) \<Longrightarrow> Is_tstack xs \<Longrightarrow> P (Abs_tstack (x#xs))"
+shows "P s"
+proof (induct s)
+  case (Abs_tstack y)
+  thus ?case 
+  using assms
+  proof (induct rule: Is_tstack_induct)
+    case (Is_tstack)
+    thus ?case using Abs_tstack by auto
+  qed auto
+qed 
+
+
+fun lookup :: "('var,'val,'a) stack \<Rightarrow> 'var \<Rightarrow> 'val" where 
   "lookup [] v = undefined" |
   "lookup (f#fs) v = (if v \<in> frame_cap f then (case (frame_st f v) of None \<Rightarrow> lookup fs v | Some x \<Rightarrow> x) else lookup fs v)"
 (* it is important that lookup ignores values from frames where v is not captured. *)
   
-fun update :: "('var,'val) stack \<Rightarrow> 'var \<Rightarrow> 'val \<Rightarrow> ('var,'val) stack" where 
+fun update :: "('var,'val,'a) stack \<Rightarrow> 'var \<Rightarrow> 'val \<Rightarrow> ('var,'val,'a) stack" where 
   "update [] _ _ = undefined" |
   "update (f#fs) v x = (if (v \<in> frame_cap f) then (f\<lparr>frame_st := (frame_st f)(v \<mapsto> x)\<rparr>)#fs else f#update fs v x)"
 
-definition tlookup :: "('var,'val) tstack \<Rightarrow> 'var \<Rightarrow> 'val" where 
+definition tlookup :: "('var,'val,'a) tstack \<Rightarrow> 'var \<Rightarrow> 'val" where 
   "tlookup fs v = lookup (Rep_tstack fs) v"
-
-lemma Pred_tstack_ConsI [intro]: "Pred_tstack xs \<Longrightarrow> Pred_tstack (x#xs)" 
-  by auto
-
-lemma Pred_tstack_ConsE [intro]: "xs \<noteq> [] \<Longrightarrow> Pred_tstack (x#xs) \<Longrightarrow> Pred_tstack xs" 
-  by auto
   
-definition tupdate :: "('var,'val) tstack \<Rightarrow> 'var \<Rightarrow> 'val \<Rightarrow> ('var,'val) tstack" where 
+definition tupdate :: "('var,'val,'a) tstack \<Rightarrow> 'var \<Rightarrow> 'val \<Rightarrow> ('var,'val,'a) tstack" where 
   "tupdate fs v x = Abs_tstack (update (Rep_tstack fs) v x)"
 
-lemma [intro!, simp]: "Is_tstack x" 
-  by induct (simp add: Abs_tstack_inverse)
+definition taux :: "('var,'val,'a) tstack \<Rightarrow> 'a" where 
+  "taux s = more (last (Rep_tstack s))"
 
-lemma Pred_tstack_update [intro!,simp]: "Pred_tstack (update (Rep_tstack fs) v x)" 
-apply (induct fs; simp only: Abs_tstack_inverse)
-proof (goal_cases)
-  case (1 y)
-  then show ?case 
-  proof (induct y rule: list.induct)
-    case (Cons x1 x2)
-    then show ?case by (cases x2) auto
-  qed auto
-qed
+definition auxupd where 
+  "auxupd s f = butlast s @ [(last s)\<lparr> more := f s \<rparr>]"
+  
+definition tauxupd :: "('var,'val,'a) tstack \<Rightarrow> (('var,'val,'a) tstack \<Rightarrow> 'a) \<Rightarrow> ('var,'val,'a) tstack" where 
+  "tauxupd s f = Abs_tstack (auxupd (Rep_tstack s) (\<lambda>x. f (Abs_tstack x)))"
+
+lemma [intro!, simp]: "Is_tstack (Rep_tstack s)" 
+using Rep_tstack by auto
+
+lemma Is_tstack_update: 
+  assumes "Is_tstack s"
+  shows "Is_tstack (update s v x)" 
+proof (induct s rule: Is_tstack_induct)
+  case (Base x)
+  then show ?case unfolding Is_tstack_def by simp
+qed (auto simp add: assms)
+
+lemma Is_tstack_update2 [intro!,simp]: "Is_tstack (update (Rep_tstack fs) v x)" 
+by (simp add: Is_tstack_update)
+
+lemma Is_tstack_upd_len: "Is_tstack s \<Longrightarrow> length (update s v x) = length s" 
+proof (induct s)
+  case (Cons a s)
+  then show ?case
+  proof (cases "v \<in> frame_cap a")
+    case False
+    have "Is_tstack s"
+    using False Cons.prems by (rule Is_tstack_notcap)
+    then show ?thesis 
+      by (simp add: False Cons)
+  qed auto  
+qed auto
+
+lemma Is_tstack_auxupd [intro]: 
+assumes "Is_tstack s" 
+shows "Is_tstack (auxupd s f)"
+apply (induct s rule: Is_tstack_induct)
+using assms unfolding Is_tstack_def auxupd_def by auto
+  
 
 find_theorems lookup
 thm ext
 
 lemma lookup_fun_upd: 
-  assumes "Pred_tstack s"
+  assumes "Is_tstack s"
   shows "lookup (update (s) var val) = (lookup s)(var := val)" 
 using assms
 proof (intro ext; induct s)
-  case Nil
-  then show ?case by simp
-next
   case (Cons a s)
   then show ?case
   proof (cases "var \<in> frame_cap a")
     case False
-    have "s \<noteq> []"
-      using False Cons.prems by auto
-    hence "Pred_tstack s" 
-      using Pred_tstack_ConsE Cons.prems by (cases s) auto
+    hence "Is_tstack s" 
+      using Is_tstack_notcap Cons.prems by auto
     thus ?thesis
       using Cons by (cases "frame_st a x") auto
   qed auto
-qed
+qed auto
 
 lemma lookup_update2:
-  assumes "Pred_tstack s"
+  assumes "Is_tstack s"
   shows  "lookup (update (s) var val) var2 = (if var2 = var then val else lookup (s) var2)"
 using lookup_fun_upd assms
 by fastforce
@@ -114,24 +204,140 @@ by fastforce
 find_theorems Abs_tstack
   
 thm type_definition_tstack
-  
+term more 
+
+lemma aux_update: 
+  shows "Is_tstack s \<Longrightarrow> more (last (update s v x)) = more (last s)"
+proof (induct s)
+  case (Cons a s)
+  then show ?case 
+  proof (cases "v \<in> frame_cap a")
+    case False
+    have s: "Is_tstack s"
+      using False Cons.prems by (rule Is_tstack_notcap)
+    hence "s \<noteq> []" by auto
+    moreover hence "update s v x \<noteq> []"
+      using Is_tstack_upd_len s length_0_conv by metis 
+    moreover have "more (last (update s v x)) = more (last (s))"
+      using Cons s by simp
+    ultimately show ?thesis by simp    
+  qed auto
+qed auto
+
+lemma auxupd_Cons [simp]:
+  "Is_tstack xs \<Longrightarrow> auxupd (x#xs) f = x # auxupd xs f"
+unfolding auxupd_def 
+apply auto 
+sledgehammr
+(* OH NO DOES NOT WORK WITH CONS DUE TO PARAM OF F*)
+
+
+lemma tauxupd_id [simp]: 
+  "tauxupd s taux = s"
+unfolding tauxupd_def taux_def auxupd_def
+using Rep_tstackI(1)[of s]
+by (induct s) (auto simp add: Abs_tstack_inverse)
+
+lemma taux_tupd [simp]: 
+  "taux (tupdate s v x) = taux s" 
+unfolding taux_def tupdate_def
+proof (induct s rule: tstack_induct)
+  case (Base x)
+  then show ?case
+    using RepAbs_id[OF Base] RepAbs_id[OF Is_tstack_update[OF Base]] aux_update 
+    by auto
+next
+  case (Frame x xs)
+  then show ?case
+  using aux_update by fastforce
+qed  
+
+
 interpretation stack: state
   "tlookup"
   tupdate
-  "\<lambda>x. ()" 
-  "\<lambda>x y. x"
-  "\<lambda>x. ()" 
+  "taux" 
+  "tauxupd"
+  "id" 
 proof (unfold_locales, goal_cases)
   case (1 s var val var2)
-  have "Pred_tstack (Rep_tstack s)" by simp
-  hence "lookup (update (Rep_tstack s) var val) var2 = (if var2 = var then val else lookup (Rep_tstack s) var2)" 
-    using lookup_update2[of "Rep_tstack s"] by simp 
+  have "lookup (update (Rep_tstack s) var val) var2 = (if var2 = var then val else lookup (Rep_tstack s) var2)" 
+    using lookup_update2[of "Rep_tstack s"] by simp
   moreover have "Rep_tstack (Abs_tstack (update (Rep_tstack s) var val)) = update (Rep_tstack s) var val" 
-    using Abs_tstack_inverse Pred_tstack_update by blast
+    using Abs_tstack_inverse Is_tstack_update by blast
   ultimately show ?case 
-    unfolding tlookup_def tupdate_def by simp
-qed (metis (full_types) unit.exhaust)+
+  unfolding tlookup_def tupdate_def by simp
+next                                          
+  case (2 s v x)
+  then show ?case 
+  proof (induct s rule: tstack_induct)
+    case (Base x')
+    hence "RepAbs_tstack [x'] = [x']" by auto
+    moreover have "Is_tstack (update [x'] v x)" using Is_tstack_update[OF Base].
+    moreover hence "RepAbs_tstack (update [x'] v x) = update [x'] v x" by auto
+    ultimately show ?case 
+      unfolding taux_def tupdate_def using Base 
+      by auto
+  next
+    case (Frame x xs)
+    then show ?case
+    by (metis Abs_tstack_inverse CollectI Is_tstack_ConsI Is_tstack_update aux_update id_apply taux_def tupdate_def)
+  qed
+next
+  case (3 s f)
+  then show ?case 
+  proof (induct s rule: tstack_induct)
+    case (Base x)
+    hence auxupd: "Is_tstack (auxupd [x] (\<lambda>x. f (Abs_tstack x)))" by auto
+    have "more (last (auxupd [x] (\<lambda>x. f (Abs_tstack x)))) = f (Abs_tstack [x])"
+      unfolding auxupd_def by auto
+    then show ?case
+      unfolding taux_def tauxupd_def by (simp add: Base auxupd)
+  next
+    case (Frame x xs)
+    hence "Is_tstack (x#xs)" by auto
+    moreover hence "RepAbs_tstack (x#xs) = x#xs" by auto
+    moreover have "Is_tstack (auxupd (x#xs) (\<lambda>x. f (Abs_tstack x)))" using Frame by auto
+    ultimately show ?case unfolding taux_def tauxupd_def auxupd_def by auto
+  qed
+next
+  case (4 s f v)
+  then show ?case 
+  proof (induct s rule: tstack_induct)
+    case (Base x)
+    moreover hence "Is_tstack (auxupd [x] (\<lambda>x. f (Abs_tstack x)))" by auto
+    ultimately show ?case 
+    proof (cases "frame_st x v")
+      case None
+      hence False using Base by blast
+      then show ?thesis by simp 
+    next
+      case (Some a)
+      then show ?thesis 
+        unfolding tlookup_def tauxupd_def 
+        using Base Is_tstack_auxupd 
+        by (auto simp add: Is_tstack_def auxupd_def)
+    qed
+  next
+    case (Frame x xs)
+    moreover hence 1: "Is_tstack (x#xs)" by auto  
+    moreover hence 2: "Is_tstack (auxupd (x # xs) (\<lambda>x. f (Abs_tstack x)))" by auto
+    moreover have 3: "lookup ( (auxupd ( xs) (\<lambda>x. f (Abs_tstack x)))) v = lookup ( xs) v"
+      using 1 2 Frame unfolding tlookup_def tauxupd_def
+      by (simp add: Is_tstack_auxupd)
+    moreover hence " lookup ( (auxupd ( (x # xs)) (\<lambda>x. f (Abs_tstack x)))) v = lookup ( (x # xs)) v" 
+    apply (cases "frame_st x v")
+    apply auto
+    apply auto
+    using Frame(1) 1 2
+    
+    
+    
 
-  
+  qed 
+qed 
+
+thm list.induct
+
 end
 
